Geb/Prototypes/Computability/Oitavem.lean
@@ -19,6 +19,7 @@ public import Geb.Prototypes.Computability.Oitavem.Machine.Read
 public import Geb.Prototypes.Computability.Oitavem.Machine.While
 public import Geb.Prototypes.Computability.Oitavem.Machine.CountOutput
 public import Geb.Prototypes.Computability.Oitavem.Machine.ReadOutput
+public import Geb.Prototypes.Computability.Oitavem.Machine.Generated
 public import Geb.Prototypes.Computability.Oitavem.Machine.Repeat
 meta import GebMeta -- shake: keep
 
